verify/Directed.v
@@ -1,0 +1,27 @@
+(** * Directed: the "head between tape cells" formulation *)
+
+From Coq Require Import Bool.
+From Coq Require Import Lists.List. Import ListNotations.
+From BusyCoq Require Export Flip.
+Set Default Goal Selector "!".
+
+Module Directed (Ctx : Ctx).
+  Module Flip := Flip Ctx. Export Flip.
+
+Definition dtape : Type := dir * list Sym * list Sym.
+
+Definition undir (d : dtape) : ctape :=
+  match d with
+  | (L, l, r) =>
+    match l with
+    | s :: l => l {{s}} r
+    | [] => [] {{s0}} r
+    end
+  | (R, l, r) =>
+    match r with
+    | s :: r => l {{s}} r
+    | [] => l {{s0}} []
+    end
+  end.
+
+End Directed.
