verify/Subtape.v
@@ -1,0 +1,115 @@
+(** * Subtape: computing the behavior on a segment of the tape *)
+
+From Coq Require Import Bool.
+From Coq Require Import Lists.List. Import ListNotations.
+From BusyCoq Require Export Directed.
+Set Default Goal Selector "!".
+
+Module Subtape (Ctx : Ctx).
+  Module Directed := Directed Ctx. Export Directed.
+
+(** We use the directional formulation here, so that
+    "the tape just got outside the segment" is easy to represent. *)
+Notation subtape := (dir * list Sym * list Sym)%type.
+
+Notation subconf := (Q * subtape)%type.
+
+Definition sublift (c : subtape) (ll rr : list Sym) : dtape :=
+  match c with
+  | (d, l, r) => (d, l ++ ll, r ++ rr)
+  end.
+
+Definition substep_at (tm : TM) (q : Q) (s : Sym) (l r : list Sym)
+    : option subconf :=
+  match tm (q, s) with
+  | Some (s', L, q') => Some (q';; (L, l, s' :: r))
+  | Some (s', R, q') => Some (q';; (R, s' :: l, r))
+  | None => None
+  end.
+
+Lemma undir_left : forall l s r, undir (L, l, s :: r) = left (l {{s}} r).
+Proof. destruct l; reflexivity. Qed.
+
+Lemma undir_right : forall l s r, undir (R, s :: l, r) = right (l {{s}} r).
+Proof. destruct l; reflexivity. Qed.
+
+Lemma step_left_lift : forall tm q q' s s' l r,
+  tm (q, s) = Some (s', L, q') ->
+  lift (q;; l {{s}} r) -[ tm ]-> lift (q';; left (l {{s'}} r)).
+Proof.
+  introv H.
+  unfold lift. rewrite lift_left.
+  exact (step_left H).
+Qed.
+
+Lemma step_right_lift : forall tm q q' s s' l r,
+  tm (q, s) = Some (s', R, q') ->
+  lift (q;; l {{s}} r) -[ tm ]-> lift (q';; right (l {{s'}} r)).
+Proof.
+  introv H.
+  unfold lift. rewrite lift_right.
+  exact (step_right H).
+Qed.
+
+Lemma substep_at_some : forall tm q s l r q' t' ll rr,
+  substep_at tm q s l r = Some (q';; t') ->
+  lift (q;; (l ++ ll) {{s}} (r ++ rr)) -[ tm ]->
+    lift (q';; undir (sublift t' ll rr)).
+Proof.
+  introv H. unfold substep_at in H.
+  destruct (tm (q, s)) as [[[s' []] q''] |] eqn:Etm; inverts H;
+   unfold sublift; simpl app.
+  - rewrite undir_left. apply step_left_lift. assumption.
+  - rewrite undir_right. apply step_right_lift. assumption.
+Qed.
+
+Definition substep (tm : TM) (c : subconf) : option subconf :=
+  match c with
+  | q;; (L, l, r) =>
+    match l with
+    | s :: l => substep_at tm q s l r
+    | [] => None
+    end
+  | q;; (R, l, r) =>
+    match r with
+    | s :: r => substep_at tm q s l r
+    | [] => None
+    end
+  end.
+
+Arguments substep : simpl never.
+
+Lemma substep_some : forall tm q q' t t' ll rr,
+  substep tm (q, t) = Some (q', t') ->
+  lift (q;; undir (sublift t ll rr)) -[ tm ]->
+    lift (q';; undir (sublift t' ll rr)).
+Proof with try discriminate; apply substep_at_some; assumption.
+  introv H. destruct t as [[[] l] r]; simpl in H.
+  - destruct l...
+  - destruct r...
+Qed.
+
+Local Hint Resolve substep_some : core.
+
+Fixpoint submultistep (tm : TM) (n : nat) (c : subconf) : option subconf :=
+  match n with
+  | 0 => Some c
+  | S n =>
+    match substep tm c with
+    | Some c' => submultistep tm n c'
+    | None => None
+    end
+  end.
+
+Lemma submultistep_some : forall tm n q q' t t' ll rr,
+  submultistep tm n (q, t) = Some (q', t') ->
+  lift (q;; undir (sublift t ll rr)) -[ tm ]->*
+    lift (q';; undir (sublift t' ll rr)).
+Proof.
+  induction n; introv H.
+  - inverts H. auto.
+  - simpl in H. destruct (substep tm (q, t)) as [[] |] eqn:E; try discriminate.
+    eauto.
+Qed.
+
+End Subtape.
